proof.v
@@ -1,20 +1,19 @@
-From iris.algebra Require Import frac dec_agree.
+From iris.algebra Require Import frac dec_agree gmap upred_big_op.
 From iris.program_logic Require Export invariants ghost_ownership.
 From iris.program_logic Require Import ownership auth.
 From iris.proofmode Require Import weakestpre tactics.
-From iris.program_logic Require Export global_functor.
 From iris.proofmode Require Import invariants ghost_ownership.
 From iris.heap_lang Require Import proofmode notation.
 From iris.heap_lang Require Export lifting heap notation.
 From iris.heap_lang.lib Require Import par.
+From iris.program_logic Require Import cancelable_invariants.
 Import uPred.
 
 From iris_spanning_tree Require Import graph mon spanning.
 
 Section wp_span.
-  Context {Σ} {Ih : heapG Σ} {iSp : spawnG Σ}
-          {IGm : authG heap_lang Σ markingUR} {IGi : inG heap_lang Σ invtokUR}
-          {IGg : authG heap_lang Σ graphUR}.
+  Context `{Ih : heapG Σ, Icnv : cinvG Σ} {ImG : authG Σ markingUR}
+          {IgG : authG Σ graphUR} {iSp : spawnG Σ}.
 
   Local Opaque span.
 
@@ -26,7 +25,7 @@ Section wp_span.
                  ∃ (m : loc), Mrk !! l = Some m ★ l ↦ (#m, (ND_to_heap v).2)
                                               ★ m ↦ (ND_to_heap v).1))
       ⊢
-      WP (span (SOME #l));; #()
+      WP (span (SOME #l))
       {{ _, ∃ g' (gtr : tree g' (λ _, true) l),
            ([★ map] l ↦ v ∈ g',
             ∃ (m : loc), Mrk !! l = Some m ★ l ↦ (#m, (ND_to_heap v).2)
@@ -35,20 +34,17 @@ Section wp_span.
       }}.
   Proof.
     iIntros (Hgnm Hgcn Hgsl) "[#Hheap Hgr]".
-    iPvs (graph_ctx_alloc with "[Hgr]") as (Im Ig Ii) "(key & #Hgr & Hg)";
+    iVs (graph_ctx_alloc with "[Hgr]") as (Ig κ) "(key & #Hgr & Hg)";
       eauto.
-    wp_focus (span _).
     iApply wp_pvs.
     iApply wp_wand_l; iSplitR;
-      [|iApply ((rec_wp_span _ _ _ _ (SOMEV #l)) with "[Hg key]"); eauto;
-        iFrame "Hheap Hgr"; by iFrame].
+      [|iApply ((rec_wp_span κ g Mrk 1 1 (SOMEV #l)) with "[Hg key]"); eauto;
+        iFrame "#"; by iFrame].
     iIntros (v) "[H key]".
-    unfold graph_ctx. iInv graphN as "Hinv".
-    iDestruct (UnPack_later with "[Hinv key]") as "[Hinv key]";
-      [iNext; iSplitL "key"; by iFrame|].
-    iPvsIntro. iSplitL "key".
-    { iNext. iApply (Dispose with "key"). }
-    wp_seq. iPvsIntro.
+    unfold graph_ctx.
+    iVs (cinv_cancel ⊤ graphN κ (graph_inv g Mrk) with "[#] [key]") as ">Hinv";
+      first done; try by iFrame.
+    iClear "Hgr". unfold graph_inv.
     iDestruct "Hinv" as (γ) "Hinv";
       iDestruct "Hinv" as (mr) "(Hi1 & Hi2 & Hi3 & Hi4 & Hi5 & Hi6)".
     iDestruct "Hi4" as %Hi4. iDestruct "Hi5" as %Hi5. iDestruct "Hi6" as %Hi6.
@@ -58,7 +54,7 @@ Section wp_span.
       iDestruct "H2" as (γ' gtr) "(Hl1 & Hl2 & Hl3)". iDestruct "Hl2" as %Hl2.
       iDestruct (whole_frac with "[Hi1 Hl1]") as "(Hi1 & Hl1 & %)";
         [by iFrame|]; subst.
-      iDestruct (marked_is_marked_in_auth with "[Hi2 Hl3]") as %Hmrk;
+      iDestruct (marked_is_marked_in_auth_sepS with "[Hi2 Hl3]") as %Hmrk;
         [by iFrame|].
       iDestruct (own_graph_valid with "Hl1") as "[Hl1 %]".
       iExists (of_graph g γ'). unshelve iExists _.
@@ -66,10 +62,19 @@ Section wp_span.
         destruct gtr as [[? ?] ?].
         rewrite of_graph_dom; trivial.
         eapply (maximally_marked_dom_marked g); eauto.
-        - (* use a lemma !*)
-          admit.
+        - apply of_graph_unmarked_orig.
         - by rewrite -{2}Hi4. }
-      by iFrame.
-  Admitted.
+        by iFrame.
+    - iDestruct "H" as "(_ & [H|H] & Hx)".
+      + iDestruct "H" as %Heq. inversion Heq.
+      + iDestruct "H" as (l') "(_ & Hl)".
+        iDestruct (marked_is_marked_in_auth with "[Hi2 Hl]") as %Hmrk;
+          [by iFrame|].
+        iDestruct (whole_frac with "[Hi1 Hx]") as "(Hi1 & Hx & %)";
+        [by iFrame|]; subst.
+        exfalso; revert Hmrk.
+        erewrite Hi4, <-to_unmarked_graph; eauto; rewrite from_to_graph //= Hgnm.
+        inversion 1.
+  Qed.
 
 End wp_span.
