spanning.v
@@ -1,12 +1,12 @@
-From iris.algebra Require Import frac dec_agree.
+From iris.algebra Require Import frac dec_agree gmap upred_big_op.
 From iris.program_logic Require Export invariants ghost_ownership.
 From iris.program_logic Require Import ownership auth.
 From iris.proofmode Require Import weakestpre tactics.
-From iris.program_logic Require Export global_functor.
 From iris.proofmode Require Import invariants ghost_ownership.
 From iris.heap_lang Require Import proofmode notation.
 From iris.heap_lang Require Export lifting heap notation.
 From iris.heap_lang.lib Require Import par.
+From iris.program_logic Require Import cancelable_invariants.
 Import uPred.
 
 From iris_spanning_tree Require Import graph mon.
@@ -36,117 +36,105 @@ Definition span : val :=
       #false
   end.
 
-  (* This change should happen in iris. -- to allow _ in the context with
-which we are binding. *)
-  Local Tactic Notation "wp_bind" open_constr(K) :=
-  lazymatch eval hnf in K with
-  | [] => idtac
-  | _ => etrans; [|fast_by apply (wp_bind K)]; simpl
-  end.
-
-  Ltac open_graph_inv Hinv key γ mr pat :=
-    let HIK := eval cbv in ("[" +:+ Hinv +:+ " " +:+ key +:+ "]") in
-    iDestruct (UnPack_later with HIK) as HIK;
-    [iNext; iSplitL key; by iFrame|];
-    rewrite {2}/graph_inv later_exist; iDestruct Hinv as (γ) Hinv;
-    rewrite later_exist; iDestruct Hinv as (mr) Hinv;
-    iDestruct Hinv as pat.
-
-
 Section Helpers.
-  Context {Σ} {Ih : heapG Σ} {Im : markingG Σ} {Ig : graphG Σ} {Ii : invtokG Σ}
-          {iSp : spawnG Σ}.
+  Context `{heapG Σ, cinvG Σ, graphG Σ, spawnG Σ} (κ : gname).
 
   Lemma wp_try_mark g Mrk k q (x : loc) :
     x ∈ dom (gset _) g →
     marked g = ∅ →
-    (heap_ctx ★ graph_ctx g Mrk ★ Γρ(q, ∅) ★ κ(k))
+    (heap_ctx ★ graph_ctx κ g Mrk ★ Γρ(q, ∅) ★ cinv_own κ k)
       ⊢
       WP (try_mark #x)
       {{ v,
          (v = #true ★
                (∃ u, ((g !! x) = Some (false, u))
-                       ★ Γρ(q, x [↦] u)) ★ μ(x) ★ κ(k))
-           ∨ (v = #false ★ Γρ(q, ∅) ★ μ(x) ★ κ(k))
+                       ★ Γρ(q, x [↦] u)) ★ μ(x) ★ cinv_own κ k)
+           ∨ (v = #false ★ Γρ(q, ∅) ★ μ(x) ★ cinv_own κ k)
       }}.
   Proof.
     iIntros (Hgx Hgnm) "(#Hheap & #Hgr & Hx & key)". unfold try_mark.
-    wp_let; wp_focus (! _)%E. unfold graph_ctx; iInv graphN as "Hinv".
-    open_graph_inv "Hinv" "key" γ mr "(Hi1 & Hi2 & Hi3 & Hi4 & Hi5 & Hi6)".
-    iDestruct (@graph_open_later with "[Hi1 Hi3]") as
+    wp_let; wp_bind (! _)%E. unfold graph_ctx.
+    iVs (cinv_open _ graphN with "Hgr key")
+      as "(>Hinv & key & Hclose)"; first done.
+    unfold graph_inv at 2.
+    iDestruct "Hinv" as (γ mr) "(Hi1 & Hi2 & Hi3 & Hi4 & Hi5 & Hi6)".
+    iDestruct (graph_open with "[Hi1 Hi3]") as
         "(Hi1 & Hi3 & Hil)"; eauto; [by iFrame|].
-    rewrite later_exist. iDestruct "Hil" as (u) "[Hil1 Hil2]".
-    rewrite later_exist. iDestruct "Hil2" as (m) "[Hil2 [Hil3 Hil4]]".
-    wp_load; iPvsIntro. iDestruct "Hil1" as %Hil1. iDestruct "Hil2" as %Hil2.
+    iDestruct "Hil" as (u) "[Hil1 Hil2]".
+    iDestruct "Hil2" as (m) "[Hil2 [Hil3 Hil4]]".
+    wp_load.
+    iDestruct "Hil1" as %Hil1. iDestruct "Hil2" as %Hil2.
     iDestruct (graph_close with "[Hi3 Hil3 Hil4]") as "Hi3";
       eauto. iFrame. iExists _; eauto. iSplitR; eauto. by iExists _; iFrame.
-    iSplitL "Hi1 Hi2 Hi3 Hi5 Hi6 Hi4".
-    { iNext. iApply Pack. iExists _, _; iFrame; auto. }
-    destruct u as [bu lu]; simpl. wp_focus (Fst _). iApply wp_fst; eauto.
+    iVs ("Hclose" with "[Hi1 Hi2 Hi3 Hi5 Hi6 Hi4]") as "_".
+    { iNext. unfold graph_inv at 2. iExists _, _; iFrame; auto. }
+    iVsIntro.
+    destruct u as [bu lu]; simpl. wp_bind (Fst _). iApply wp_fst; eauto.
     { by destruct lu as [[] []]; simpl; eauto. }
-    iNext; iPvsIntro; wp_let. iInv graphN as "Hinv".
-    open_graph_inv "Hinv" "key" γ' mr' "(Hi1 & Hi2 & Hi3 & Hi4 & Hi5 & Hi6)".
-    iDestruct (graph_open_later with "[Hi1 Hi3]") as
+    iNext; iVsIntro; wp_let.
+    iVs (cinv_open _ graphN with "Hgr key")
+      as "(>Hinv & key & Hclose)"; first done.
+    unfold graph_inv at 2.
+    iDestruct "Hinv" as (γ' mr') "(Hi1 & Hi2 & Hi3 & Hi4 & Hi5 & Hi6)".
+    iDestruct (graph_open with "[Hi1 Hi3]") as
         "(Hi1 & Hi3 & Hil)"; eauto; [by iFrame|].
-    rewrite later_exist. iDestruct "Hil" as (u) "[Hil1 Hil2]".
-    rewrite later_exist. iDestruct "Hil2" as (m') "[Hil2 [Hil3 Hil4]]".
-    iTimeless "Hil2". iDestruct "Hil2" as %Hil2'.
-    iTimeless "Hil1". iDestruct "Hil1" as %Hil1'.
-    iTimeless "Hi5". iDestruct "Hi5" as %Hi5.
-    iTimeless "Hi6". iDestruct "Hi6" as %Hi6.
-    iTimeless "Hi4". iDestruct "Hi4" as %Hi4.
+    iDestruct "Hil" as (u) "[Hil1 Hil2]".
+    iDestruct "Hil2" as (m') "[Hil2 [Hil3 Hil4]]".
+    iDestruct "Hil2" as %Hil2'. iDestruct "Hil1" as %Hil1'.
+    iDestruct "Hi5" as %Hi5. iDestruct "Hi6" as %Hi6. iDestruct "Hi4" as %Hi4.
     rewrite Hil2' in Hil2; inversion Hil2; subst.
     destruct u as [[] lu']; simpl in *.
-    - (* CAS fails *)
-      wp_cas_fail.
+    - wp_cas_fail.
       iDestruct (graph_close with "[Hi3 Hil3 Hil4]") as "Hi3";
-        eauto. iFrame. iExists _; eauto. iSplitR; eauto. by iExists _; iFrame.
-      iPvs (already_marked with "Hi2") as "[Hi2 Hxm]"; [|iFrame "Hxm"].
+      eauto. iFrame. iExists _; eauto. iSplitR; eauto. by iExists _; iFrame.
+      iVs (already_marked with "Hi2") as "[Hi2 Hxm]"; [|iFrame "Hxm"].
       { rewrite Hi4. eapply graph.is_marked; eauto. }
-      iPvsIntro; iFrame. iSplitR "Hx".
-      + iNext; iApply Pack.
-        unfold graph_inv; iExists _, _; iFrame; repeat iSplitL; trivial.
-      + by iRight; iFrame.
+      iVs ("Hclose" with "[Hi1 Hi2 Hi3]") as "_".
+      { iNext. unfold graph_inv at 2. iExists _, _; iFrame; auto. }
+      iVsIntro. iFrame. iRight; by iFrame.
     - (* CAS succeeds *)
       wp_cas_suc.
       iDestruct (auth_own_graph_valid with "Hi1") as "[Hi1 H]".
       iDestruct "H" as %Hv1.
-      iPvs (mark_graph _ _ x lu' with "[Hi1 Hx]") as "[Hi1 Hx]";
+      iVs (mark_graph _ _ x lu' with "[Hi1 Hx]") as "[Hi1 Hx]";
         try by iFrame. eapply unmarked_in_graph_mon; eauto.
-      iPvs (new_marked with "Hi2") as "[Hi2 Hm]". iFrame "key Hm".
+      iVs (new_marked with "Hi2") as "[Hi2 Hm]". iFrame "key Hm".
       erewrite delete_marked.
       iDestruct (auth_own_graph_valid with "Hi1") as "[Hi1 %]".
       iDestruct (graph_close with "[Hi3 Hil3 Hil4]") as "Hi3".
       { iFrame. iExists (_, _). iSplitR; [| iExists _; by iFrame].
           by rewrite mark_update_lookup. }
       pose proof (unmarked_from_g _ _ _ _ Hv1 Hil1') as Hfg.
-      iPvsIntro. iSplitR "Hx".
-      + iNext; iApply Pack; unfold graph_inv. iExists _, _; iFrame.
+      iVs ("Hclose" with "[Hi1 Hi2 Hi3]") as "_".
+      + iNext; unfold graph_inv at 2. iExists _, _; iFrame.
         repeat iSplit; iPureIntro.
         { by rewrite new_marking_dom marking_union //= Hi4. }
         { erewrite mark_dom_union => i. rewrite elem_of_union elem_of_singleton.
           intros [?|?]; subst; auto. }
         { apply agrees_op; trivial; split; eauto using nodes_agree_refl. }
-      + iLeft; iSplit; trivial. iExists _; by iFrame.
+      + iVsIntro. iLeft; iSplit; trivial. iExists _; by iFrame.
   Qed.
 
   Lemma wp_load_graph g Mrk k q (x : loc) u w :
     (g !! x) = Some (false, u) →
-    (heap_ctx ★ graph_ctx g Mrk ★ Γρ(q, x [↦] w) ★ κ(k))
+    (heap_ctx ★ graph_ctx κ g Mrk ★ Γρ(q, x [↦] w) ★ cinv_own κ k)
       ⊢
       WP (! #x)
       {{ v, (∃ m : loc, (Mrk !! x) = Some m ∧ v = (#m, pr_opl_heap w)%V)
-              ★ ■ node_agrees w u ★ Γρ(q, x [↦] w) ★ κ(k) }}.
+              ★ ■ node_agrees w u ★ Γρ(q, x [↦] w) ★ cinv_own κ k }}.
   Proof.
     iIntros (Hgx) "(#Hheap & #Hgr & Hx & key)".
     assert (Hgx' : x ∈ dom (gset _) g).
     { rewrite elem_of_dom Hgx; eauto. }
-    unfold graph_ctx; iInv graphN as "Hinv".
-    open_graph_inv "Hinv" "key" γ mr "(Hi1 & Hi2 & Hi3 & Hi4 & Hi5 & Hi6)".
-    iDestruct (graph_open_later with "[Hi1 Hi3]")
-      as "(Hi1 & Hi3 & Hil)"; eauto; [by iFrame|].
-    rewrite later_exist. iDestruct "Hil" as (o) "[Hil1 Hil2]".
-    rewrite later_exist. iDestruct "Hil2" as (m) "[Hil2 [Hil3 Hil4]]".
+    unfold graph_ctx.
+    iVs (cinv_open _ graphN with "Hgr key")
+      as "(>Hinv & key & Hclose)"; first done.
+    unfold graph_inv at 2.
+    iDestruct "Hinv" as (γ mr) "(Hi1 & Hi2 & Hi3 & Hi4 & Hi5 & Hi6)".
+    iDestruct (graph_open with "[Hi1 Hi3]") as
+        "(Hi1 & Hi3 & Hil)"; eauto; [by iFrame|].
+    iDestruct "Hil" as (u') "[Hil1 Hil2]".
+    iDestruct "Hil2" as (m) "[Hil2 [Hil3 Hil4]]".
     wp_load. iDestruct "Hi5" as %Hi5. iDestruct "Hil1" as %Hil1.
     iDestruct "Hil2" as %Hil2. iDestruct "Hi6" as %Hi6. iDestruct "Hi4" as %Hi4.
     iDestruct (auth_own_graph_valid with "Hi1") as "[Hi1 Hvγ]".
@@ -156,11 +144,10 @@ Section Helpers.
     rewrite mark_update_lookup in Hil1'; trivial.
     iDestruct (graph_close with "[Hi3 Hil3 Hil4]") as "Hi3"; [iFrame|].
     { iExists _; iSplitR; auto. iExists _; by iFrame. }
-    iPvsIntro. iSplitL "Hi1 Hi2 Hi3".
-    { iNext; iApply Pack. unfold graph_inv at 2.
-      iExists _, _; iFrame; repeat iSplit; by iPureIntro. }
-    iFrame. inversion Hil1'; subst o; simpl.
-    iSplit; [|iPureIntro]. iExists _; iSplit; by iPureIntro.
+    iVs ("Hclose" with "[Hi1 Hi2 Hi3]") as "_".
+    { iNext. unfold graph_inv at 2. iExists _, _; iFrame; auto. }
+    iFrame. inversion Hil1'; subst u'; simpl.
+    iVsIntro. iSplit; [|iPureIntro]. iExists _; iSplit; by iPureIntro.
     { rewrite Heq in Hi6.
       specialize (Hi6 x w).
       destruct Hi6 as [u' [Hi61 Hi62]].
@@ -177,20 +164,23 @@ Section Helpers.
       node_agrees w' v →
       (Mrk !! x) = Some m →
       (g !! x) = Some (false, v) →
-      (heap_ctx ★ graph_ctx g Mrk ★ Γρ(q, x [↦] w) ★ κ(k))
+      (heap_ctx ★ graph_ctx κ g Mrk ★ Γρ(q, x [↦] w) ★ cinv_own κ k)
         ⊢
         WP (#x <- (#m, pr_opl_heap w'))
-        {{ v, Γρ(q, x [↦] w') ★ κ(k) }}.
+        {{ v, Γρ(q, x [↦] w') ★ cinv_own κ k }}.
   Proof.
     iIntros (Hagree Hmrk Hgx) "(#Hheap & #Hgr & Hx & key)".
     assert (Hgx' : x ∈ dom (gset _) g).
     { rewrite elem_of_dom Hgx; eauto. }
-    unfold graph_ctx; iInv graphN as "Hinv".
-    open_graph_inv "Hinv" "key" γ mr "(Hi1 & Hi2 & Hi3 & Hi4 & Hi5 & Hi6)".
-    iDestruct (graph_open_later with "[Hi1 Hi3]")
-      as "(Hi1 & Hi3 & Hil)"; eauto; [by iFrame|].
-    rewrite later_exist. iDestruct "Hil" as (u) "[Hil1 Hil2]".
-    rewrite later_exist. iDestruct "Hil2" as (m') "[Hil2 [Hil3 Hil4]]".
+    unfold graph_ctx.
+    iVs (cinv_open _ graphN with "Hgr key")
+      as "(>Hinv & key & Hclose)"; first done.
+    unfold graph_inv at 2.
+    iDestruct "Hinv" as (γ mr) "(Hi1 & Hi2 & Hi3 & Hi4 & Hi5 & Hi6)".
+    iDestruct (graph_open with "[Hi1 Hi3]") as
+        "(Hi1 & Hi3 & Hil)"; eauto; [by iFrame|].
+    iDestruct "Hil" as (u') "[Hil1 Hil2]".
+    iDestruct "Hil2" as (m') "[Hil2 [Hil3 Hil4]]".
     wp_store.
     iDestruct "Hil2" as %Hil2.
     rewrite Hmrk in Hil2. inversion Hil2; subst; clear Hil2.
@@ -200,9 +190,9 @@ Section Helpers.
     iDestruct "Hvγ" as %Hvγ. iDestruct (graph_pointsto_marked with "[Hi1 Hx]")
       as "(Hi1 & Hx & Heq)"; try by iFrame.
     pose proof Hil1 as Hil1'. iDestruct "Heq" as %Heq; rewrite Heq in Hil1' Hvγ.
-    rewrite mark_update_lookup in Hil1'; trivial. inversion Hil1'; subst u.
+    rewrite mark_update_lookup in Hil1'; trivial. inversion Hil1'; subst u'.
     clear Hil1'. simpl. rewrite Heq.
-    iPvs (update_graph _ _ _ w' with "[Hi1 Hx]") as
+    iVs (update_graph _ _ _ w' with "[Hi1 Hx]") as
         "[Hi1 Hx]"; try by iFrame. by rewrite lookup_delete.
     rewrite -delete_marked. erewrite (delete_marked _ _ _ w').
     assert (Hvγ' : ✓ ({[x := Excl w']} ⋅ delete x γ)).
@@ -210,9 +200,9 @@ Section Helpers.
     iDestruct (graph_close with "[Hi3 Hil3 Hil4]") as "Hi3".
     { iFrame. iExists _. iSplitR.
       - rewrite ?mark_update_lookup; eauto. - iExists _; by iFrame. }
-    iPvsIntro; iFrame.
-    iNext. iApply Pack. unfold graph_inv at 2.
-    iExists _, _; iFrame. repeat iSplit; iPureIntro.
+    iVs ("Hclose" with "[Hi1 Hi2 Hi3]") as "_"; [|by iFrame].
+    unfold graph_inv at 2.
+    iNext. iExists _, _; iFrame. repeat iSplit; iPureIntro.
     { rewrite Heq in Hi4. rewrite Hi4 ?marking_union; trivial. }
     { rewrite mark_dom_union => i.
       rewrite elem_of_union dom_delete elem_of_singleton.
@@ -225,26 +215,26 @@ Section Helpers.
   Lemma wp_unmark_fst g Mrk k q (x : loc) v w1 w2 :
     (g !! x) = Some (false, v) →
     marked g = ∅ →
-    (heap_ctx ★ graph_ctx g Mrk ★ Γρ(q, x [↦] (w1, w2)) ★ κ(k))
+    (heap_ctx ★ graph_ctx κ g Mrk ★ Γρ(q, x [↦] (w1, w2)) ★ cinv_own κ k)
       ⊢
       WP (unmark_fst #x)
-      {{ _, Γρ(q, x [↦] (None, w2)) ★ κ(k) }}.
+      {{ _, Γρ(q, x [↦] (None, w2)) ★ cinv_own κ k }}.
   Proof.
     iIntros (Hgx Hgnm) "(#Hheap & #Hgr & Hx & key)". unfold unmark_fst.
-    wp_let. wp_focus (! _)%E.
+    wp_let. wp_bind (! _)%E.
     iApply wp_wand_l; iSplitR;
       [|iApply wp_load_graph; eauto; iFrame "Hheap Hgr"; by iFrame].
     iIntros (u) "(H1 & Hagree & Hx & key)". iDestruct "H1" as (m) "[Hmrk Hu]".
     iDestruct "Hagree" as %Hagree.
     iDestruct "Hmrk" as %Hmrk; iDestruct "Hu" as %Hu; subst.
-    wp_let. wp_focus (Fst _). iApply wp_fst; eauto.
+    wp_let. wp_bind (Fst _). iApply wp_fst; eauto.
     { rewrite to_val_pr_opl_heap'; eauto. }
-    iNext; iPvsIntro. wp_focus (Snd (_, _)). iApply wp_snd; eauto.
+    iNext; iVsIntro. wp_bind (Snd (_, _)). iApply wp_snd; eauto.
     { by rewrite to_val_pr_opl_heap'. }
-    iNext; iPvsIntro. wp_focus (Snd _). iApply wp_snd; eauto.
+    iNext; iVsIntro. wp_bind (Snd _). iApply wp_snd; eauto.
     { rewrite to_val_opl_heap; eauto. }
     {by rewrite to_val_opl_heap. }
-    iNext. iPvsIntro.
+    iNext. iVsIntro.
     iApply (wp_store_graph _ (None, w2) with "[Hx key]"); eauto;
       [|iFrame "Hheap Hgr"; by iFrame].
     { by destruct w1; destruct w2; destruct v; inversion Hagree; subst. }
@@ -253,26 +243,26 @@ Section Helpers.
   Lemma wp_unmark_snd g Mrk k q (x : loc) v w1 w2 :
     (g !! x) = Some (false, v) →
     marked g = ∅ →
-    (heap_ctx ★ graph_ctx g Mrk ★ Γρ(q, x [↦] (w1, w2)) ★ κ(k))
+    (heap_ctx ★ graph_ctx κ g Mrk ★ Γρ(q, x [↦] (w1, w2)) ★ cinv_own κ k)
       ⊢
       WP (unmark_snd #x)
-      {{ _, Γρ(q, x [↦] (w1, None)) ★ κ(k) }}.
+      {{ _, Γρ(q, x [↦] (w1, None)) ★ cinv_own κ k }}.
   Proof.
     iIntros (Hgx Hgnm) "(#Hheap & #Hgr & Hx & key)". unfold unmark_fst.
-    wp_let. wp_focus (! _)%E.
+    wp_let. wp_bind (! _)%E.
     iApply wp_wand_l; iSplitR;
       [|iApply wp_load_graph; eauto; iFrame "Hheap Hgr"; by iFrame].
     iIntros (u) "(H1 & Hagree & Hx & key)". iDestruct "H1" as (m) "[Hmrk Hu]".
     iDestruct "Hagree" as %Hagree.
     iDestruct "Hmrk" as %Hmrk; iDestruct "Hu" as %Hu; subst.
-    wp_let. wp_focus (Fst _). iApply wp_fst; eauto.
+    wp_let. wp_bind (Fst _). iApply wp_fst; eauto.
     { rewrite to_val_pr_opl_heap'; eauto. }
-    iNext; iPvsIntro. wp_focus (Snd (_, _)). iApply wp_snd; eauto.
+    iNext; iVsIntro. wp_bind (Snd (_, _)). iApply wp_snd; eauto.
     { by rewrite to_val_pr_opl_heap'. }
-    iNext; iPvsIntro. wp_focus (Fst _). iApply wp_fst; eauto.
+    iNext; iVsIntro. wp_bind (Fst _). iApply wp_fst; eauto.
     {by rewrite to_val_opl_heap. }
     { rewrite to_val_opl_heap; eauto. }
-    iNext. iPvsIntro.
+    iNext. iVsIntro.
     iApply (wp_store_graph _ (w1, None) with "[Hx key]"); eauto;
       [|iFrame "Hheap Hgr"; by iFrame].
     { by destruct w1; destruct w2; destruct v; inversion Hagree; subst. }
@@ -300,9 +290,9 @@ Section Helpers.
   Lemma self_contained_l g x b w1 w2:
     self_contained g x → g !! x = Some (b, (Some w1, w2)) → self_contained g w1.
   Proof.
-    intros H1 H2. split.
-    - apply H1; econstructor 2; eauto; constructor 1; eauto.
-    - intros y H3. apply H1. econstructor 2; eauto.
+    intros Hgsl Hgx. split.
+    - apply Hgsl; econstructor 2; eauto; constructor 1; eauto.
+    - intros y Hwp. apply Hgsl. econstructor 2; eauto.
   Qed.
 
   Hint Resolve self_contained_l.
@@ -310,9 +300,9 @@ Section Helpers.
   Lemma self_contained_r g x b w1 w2:
     self_contained g x → g !! x = Some (b, (w1, Some w2)) → self_contained g w2.
   Proof.
-    intros H1 H2. split.
-    - apply H1; econstructor 3; eauto; constructor 1; eauto.
-    - intros y H3. apply H1. econstructor 3; eauto.
+    intros Hgsl Hgx. split.
+    - apply Hgsl; econstructor 3; eauto; constructor 1; eauto.
+    - intros y Hwp. apply Hgsl. econstructor 3; eauto.
   Qed.
 
   Hint Resolve self_contained_r.
@@ -401,7 +391,6 @@ Section Helpers.
       revert Hz2; rewrite elem_of_singleton; intros Hz2;
         subst; rewrite Hgl in Hz3; inversion Hz3; subst; trivial.
   Qed.
-
 
   Lemma maximally_marked_l (g : graph loc)
         (γ1 : gmapR loc (exclR chlC)) l u1 u2 (l1 : loc)
@@ -586,7 +575,7 @@ Section Helpers.
     marked g = ∅ →
     (x = NONEV ∨ ∃ l : loc,
         x = SOMEV #l ∧ self_contained g l) →
-    (heap_ctx ★ graph_ctx g Mrk ★ ▷ Γρ(q, ∅) ★ ▷ κ(k))
+    (heap_ctx ★ graph_ctx κ g Mrk ★ Γρ(q, ∅) ★ cinv_own κ k)
       ⊢
       WP (span x)
       {{ v, ((v = # true ★
@@ -602,7 +591,7 @@ Section Helpers.
              ∨
              (v = # false ★ (x = NONEV ∨ (∃ l : loc, x = SOMEV #l ★ μ(l)))
                     ★ Γρ(q, ∅)))
-              ★ κ(k)
+              ★ cinv_own κ k
       }}.
   Proof.
     intros Hgnm Hxpt. iIntros "(#Hheap & #Hgr & Hx & key)".
@@ -610,36 +599,36 @@ Section Helpers.
     iIntros (x Hxpt k q) "key Hx".
     wp_rec.
     destruct Hxpt as [|[l [? Hgsl]]]; subst.
-    { wp_match. iPvsIntro.
+    { wp_match. iVsIntro.
       iFrame; iRight; iFrame; repeat iSplit; trivial; by iLeft. }
-    wp_match. wp_focus (try_mark _).
+    wp_match. wp_bind (try_mark _).
     iDestruct (empty_graph_divide with "Hx") as "[Hx1 Hx2]".
     iApply wp_wand_l; iSplitL "Hx1";
       [|iApply wp_try_mark; try iFrame]; eauto; simpl.
     iIntros (v) "[(% & Hv & Hm & key)|(% & Hx2 & Hm & key)]"; subst;
     [|iCombine "Hx1" "Hx2" as "Hx"; rewrite -graph_divide ucmra_unit_right_id;
-      wp_if; iPvsIntro; iFrame; iRight; iFrame; iSplit; trivial; iRight;
+      wp_if; iVsIntro; iFrame; iRight; iFrame; iSplit; trivial; iRight;
       iExists _; eauto].
     iDestruct "Hv" as (u) "[Hgl Hl]". iDestruct "Hgl" as %Hgl.
     wp_if.
     (* reading the reference. This part is very similar to unmark lemmas! *)
-    wp_focus (! _)%E.
+    wp_bind (! _)%E.
     iApply wp_wand_l; iSplitR "Hl key";
       [|iApply wp_load_graph; eauto; iFrame "Hheap Hgr"; by iFrame].
     iIntros (v) "(H1 & Hagree & Hx & key)". iDestruct "H1" as (m) "[Hmrk Hv]".
     iDestruct "Hagree" as %Hagree. iDestruct "Hv" as %Hv; subst v.
-    wp_let. wp_focus (par _).
-    iDestruct (token_divide with "key") as "[K1 K2]".
+    wp_let. wp_bind (par _).
+    erewrite <- cinv_own_half. iDestruct "key" as "[K1 K2]".
     iDestruct (empty_graph_divide with "Hx1") as "[Hx11 Hx12]".
     destruct u as [u1 u2]. iApply wp_par. iSplitR; [by iFrame "Hheap"|].
     (* symbolically executing the left part of the par. *)
     iSplitL "Hx11 K1".
-    wp_focus (Snd _). iApply wp_snd; eauto.
+    wp_bind (Snd _). iApply wp_snd; eauto.
     { by rewrite to_val_pr_opl_heap'. }
-    iNext; iPvsIntro. wp_focus (Fst _). iApply wp_fst.
+    iNext; iVsIntro. wp_bind (Fst _). iApply wp_fst.
     { by rewrite to_val_opl_heap. }
     { rewrite to_val_opl_heap; eauto. }
-    iNext; iPvsIntro.
+    iNext; iVsIntro.
     assert (Hlf : (opl_heap u1) = NONEV
                 ∨ (∃ l : loc,
                       (opl_heap u1) = SOMEV #l ∧ self_contained g l)).
@@ -648,12 +637,12 @@ Section Helpers.
     iApply ("IH" with "[#] * [K1] [Hx11]"); auto.
     (* symbolically executing the left part of the par. *)
     iSplitL "Hx12 K2".
-    wp_focus (Snd (_, _)). iApply wp_snd; eauto.
+    wp_bind (Snd (_, _)). iApply wp_snd; eauto.
     { by rewrite to_val_pr_opl_heap'. }
-    iNext; iPvsIntro. wp_focus (Snd _). iApply wp_snd.
+    iNext; iVsIntro. wp_bind (Snd _). iApply wp_snd.
     { rewrite to_val_opl_heap; eauto. }
     { by rewrite to_val_opl_heap. }
-    iNext; iPvsIntro.
+    iNext; iVsIntro.
     assert (Hrh : (opl_heap u2) = NONEV
                 ∨ (∃ l : loc,
                       (opl_heap u2) = SOMEV #l ∧ self_contained g l)).
@@ -661,19 +650,19 @@ Section Helpers.
       exists l2; split; trivial. eapply self_contained_r; eauto. }
     iApply ("IH" with "[#] * [K2] [Hx12]"); auto.
     iIntros (vl vr) "[[Hvl K1] [Hvr K2]]".
-    iCombine "K1" "K2" as "key". rewrite -token_divide.
+    iCombine "K1" "K2" as "key". rewrite cinv_own_half.
     iNext. wp_let.
     (* We don't need the huge induction hypothesis anymore. *)
     iClear "IH".
     (* separating all four cases *)
     iDestruct "Hvl" as "[[% Hvll]|[% Hvlr]]"; subst;
       iDestruct "Hvr" as "[[% Hvrl]|[% Hvrr]]"; subst.
-    - wp_focus (Fst _). iApply wp_fst; eauto. iNext; iPvsIntro.
-      wp_focus (UnOp _ _). iApply wp_un_op; first done. iNext; iPvsIntro.
+    - wp_bind (Fst _). iApply wp_fst; eauto. iNext; iVsIntro.
+      wp_bind (UnOp _ _). iApply wp_un_op; try done. iNext; iVsIntro.
       wp_if; wp_seq.
-      wp_focus (Snd _). iApply wp_snd; eauto. iNext; iPvsIntro.
-      wp_focus (UnOp _ _). iApply wp_un_op; first done.
-      iNext; iPvsIntro.
+      wp_bind (Snd _). iApply wp_snd; eauto. iNext; iVsIntro.
+      wp_bind (UnOp _ _). iApply wp_un_op; try done.
+      iNext; iVsIntro.
       wp_if.
       iDestruct "Hvll" as (l1) "(Hl1eq & Hg1 & ml1)".
       iDestruct "Hg1" as (γ1 mmr1) "[Hxl [Hl1im Hfml]]".
@@ -684,7 +673,7 @@ Section Helpers.
       iCombine "Hxl" "Hxr" as "Hxlr". rewrite -graph_divide.
       iCombine "Hx" "Hxlr" as "Hx". rewrite -graph_divide.
       rewrite dup_marked. iDestruct "Hm" as "[Hm1 Hm2]".
-      iPvsIntro. iFrame; iLeft. iSplit; [trivial|].
+      iVsIntro. iFrame; iLeft. iSplit; [trivial|].
       iExists _; iSplit; [trivial|]. iFrame.
       iDestruct (own_graph_valid with "Hx") as "[Hx %]".
       iExists ({[l := Excl (u1, u2)]} ⋅ (γ1 ⋅ γ2)).
@@ -693,12 +682,12 @@ Section Helpers.
       rewrite of_graph_singleton_op ?marked_insert ?elem_of_union
               ?elem_of_singleton; eauto.
       iApply (front_marked_lr with "*"); eauto; by iFrame.
-    - wp_focus (Fst _). iApply wp_fst; eauto. iNext; iPvsIntro.
-      wp_focus (UnOp _ _). iApply wp_un_op; first done. iNext; iPvsIntro.
+    - wp_bind (Fst _). iApply wp_fst; eauto. iNext; iVsIntro.
+      wp_bind (UnOp _ _). iApply wp_un_op; try done. iNext; iVsIntro.
       wp_if; wp_seq.
-      wp_focus (Snd _). iApply wp_snd; eauto. iNext; iPvsIntro.
-      wp_focus (UnOp _ _). iApply wp_un_op; first done.
-      iNext; iPvsIntro.
+      wp_bind (Snd _). iApply wp_snd; eauto. iNext; iVsIntro.
+      wp_bind (UnOp _ _). iApply wp_un_op; try done.
+      iNext; iVsIntro.
       wp_if.
       iDestruct "Hvll" as (l1) "(Hl1eq & Hg1 & ml1)".
       iDestruct "Hg1" as (γ1 mmr1) "[Hxl [Hl1im Hfml]]".
@@ -710,7 +699,7 @@ Section Helpers.
       iIntros (v) "[Hx key]".
       iCombine "Hx" "Hxlr" as "Hx". rewrite -graph_divide.
       rewrite dup_marked. iDestruct "Hm" as "[Hm1 Hm2]".
-      wp_value; iPvsIntro; wp_seq; iPvsIntro.
+      wp_value; iVsIntro; wp_seq; iVsIntro.
       iFrame; iLeft. iSplit; [trivial|].
       iExists _; iSplit; [trivial|]. iFrame.
       iDestruct (own_graph_valid with "Hx") as "[Hx %]".
@@ -720,8 +709,8 @@ Section Helpers.
       rewrite of_graph_singleton_op ?marked_insert ?elem_of_union
               ?elem_of_singleton; eauto.
       iApply (front_marked_l with "*"); eauto; by iFrame.
-    - wp_focus (Fst _). iApply wp_fst; eauto. iNext; iPvsIntro.
-      wp_focus (UnOp _ _). iApply wp_un_op; first done. iNext; iPvsIntro.
+    - wp_bind (Fst _). iApply wp_fst; eauto. iNext; iVsIntro.
+      wp_bind (UnOp _ _). iApply wp_un_op; try done. iNext; iVsIntro.
       wp_if.
       iDestruct "Hvlr" as "(Hvl & Hxl)".
       iDestruct "Hvrl" as (l2) "(Hl2eq & Hg2 & ml2)".
@@ -733,12 +722,12 @@ Section Helpers.
       iIntros (v) "[Hx key]".
       iCombine "Hx" "Hxlr" as "Hx". rewrite -graph_divide.
       wp_seq.
-      wp_focus (Snd _). iApply wp_snd; eauto. iNext; iPvsIntro.
-      wp_focus (UnOp _ _). iApply wp_un_op; first done.
-      iNext; iPvsIntro.
+      wp_bind (Snd _). iApply wp_snd; eauto. iNext; iVsIntro.
+      wp_bind (UnOp _ _). iApply wp_un_op; try done.
+      iNext; iVsIntro.
       wp_if.
       rewrite dup_marked. iDestruct "Hm" as "[Hm1 Hm2]".
-      iPvsIntro.
+      iVsIntro.
       iFrame; iLeft. iSplit; [trivial|].
       iExists _; iSplit; [trivial|]. iFrame.
       iDestruct (own_graph_valid with "Hx") as "[Hx %]".
@@ -751,16 +740,16 @@ Section Helpers.
     - iDestruct "Hvlr" as "(Hvl & Hxl)".
       iDestruct "Hvrr" as "(Hvr & Hxr)".
       iCombine "Hxl" "Hxr" as "Hxlr". rewrite -graph_divide ucmra_unit_right_id.
-      wp_focus (Fst _). iApply wp_fst; eauto. iNext; iPvsIntro.
-      wp_focus (UnOp _ _). iApply wp_un_op; first done. iNext; iPvsIntro.
+      wp_bind (Fst _). iApply wp_fst; eauto. iNext; iVsIntro.
+      wp_bind (UnOp _ _). iApply wp_un_op; try done. iNext; iVsIntro.
       wp_if.
       iApply wp_wand_l; iSplitR "Hx key";
         [|iApply wp_unmark_fst; eauto; by iFrame "Hgr Hheap"; iFrame].
       iIntros (v) "[Hx key]".
       wp_seq.
-      wp_focus (Snd _). iApply wp_snd; eauto. iNext; iPvsIntro.
-      wp_focus (UnOp _ _). iApply wp_un_op; first done.
-      iNext; iPvsIntro.
+      wp_bind (Snd _). iApply wp_snd; eauto. iNext; iVsIntro.
+      wp_bind (UnOp _ _). iApply wp_un_op; try done.
+      iNext; iVsIntro.
       wp_if.
       iApply wp_wand_l; iSplitR "Hx key";
         [|iApply wp_unmark_snd; eauto; by iFrame "Hgr Hheap"; iFrame].
@@ -768,7 +757,7 @@ Section Helpers.
       iCombine "Hx" "Hxlr" as "Hx". rewrite -graph_divide.
       wp_seq.
       rewrite dup_marked. iDestruct "Hm" as "[Hm1 Hm2]".
-      iPvsIntro.
+      iVsIntro.
       iFrame; iLeft. iSplit; [trivial|].
       iExists _; iSplit; [trivial|]. iFrame.
       iDestruct (own_graph_valid with "Hx") as "[Hx %]".
